Tweak exercises.

theories/exercises_answers.v
@@ -6,27 +6,30 @@ From tutorial_popl20 Require Export sem_typing safety.
 Section exercises.
   Context `{heapG Σ}.
 
-  Definition exercise1_prog : val := λ: <>, if: #true then #13 else #13 #37.
+  (* Easy *)
+  Definition exercise1_prog : val := λ: <>,
+    if: #true then #13 else #13 #37.
 
-  Lemma exercise1 : ∅ ⊨ exercise1_prog : sem_ty_unit → sem_ty_int.
+  Lemma exercise1 : ∅ ⊨ exercise1_prog : () → sem_ty_int.
   Proof.
     iIntros (vs) "!# HΓ"; simpl.
     iApply wp_value.
-    iIntros "!#" (w) "Hw".
+    iIntros "!#" (? ->).
     wp_lam.
     wp_if.
     rewrite /sem_ty_car /=.
     by iExists 13.
   Qed.
 
-  Definition exercise2_prog : val :=
-    λ: <>, let: "l" := ref #0 in "l" <- #true;; !"l".
+  (* Easy *)
+  Definition exercise2_prog : val := λ: <>,
+    let: "l" := ref #0 in "l" <- #true;; !"l".
 
-  Lemma exercise2 : ∅ ⊨ exercise2_prog : sem_ty_unit → sem_ty_bool.
+  Lemma exercise2 : ∅ ⊨ exercise2_prog : () → sem_ty_bool.
   Proof.
     iIntros (vs) "!# HΓ"; simpl.
     iApply wp_value.
-    iIntros "!#" (v) "Hv".
+    iIntros "!#" (? ->).
     wp_lam.
     wp_alloc l as "Hl".
     wp_let.
@@ -36,207 +39,149 @@ Section exercises.
     by iExists true.
   Qed.
 
-  Definition exercise3_prog : val :=
-    λ: <>,
-       let: "l" := ref #1 in
-       ((λ: "x", if: "x" ≠ #0 then "l" <- "x" else #()),
-        (λ: <>, assert: !"l" ≠ #0)).
+  (* Moderate *)
+  Definition exercise3_prog : val := λ: <>,
+    let: "l" := ref #1 in
+    ((λ: "x", if: "x" ≠ #0 then "l" <- "x" else #()),
+     (λ: <>, assert: !"l" ≠ #0)).
 
-  Lemma exercise3 :
-    ∅ ⊨ exercise3_prog :
-      sem_ty_unit → (sem_ty_int → sem_ty_unit) * (sem_ty_unit → sem_ty_unit).
+  Lemma exercise3 : ∅ ⊨ exercise3_prog : () → (sem_ty_int → ()) * (() → ()).
   Proof.
     iIntros (vs) "!# HΓ"; simpl.
     iApply wp_value.
-    iIntros "!#" (v) "Hv".
+    iIntros "!#" (? ->).
     wp_lam.
     wp_alloc l as "Hl".
     wp_let.
-    iMod (inv_alloc (nroot .@ "ex3") _ (∃ n : Z, ⌜#n ≠ #0⌝ ∗ l ↦ #n) with "[Hl]")%I
-      as "#Hinv".
+    pose (I := (∃ n : Z, ⌜#n ≠ #0⌝ ∗ l ↦ #n)%I).
+    iMod (inv_alloc (nroot .@ "exercise3") _ I with "[Hl]")%I as "#Hinv".
     { by iNext; iExists 1; iFrame. }
     wp_pures.
     iExists _, _. iSplit; first done.
     iSplit.
-    - iIntros "!#" (w) "Hw".
-      iDestruct "Hw" as (n) "%".
-      subst.
+    - iIntros "!#" (? [n ->]).
       wp_lam.
       wp_op.
-      destruct (decide (#n = #0%Z)); first subst.
-      + rewrite bool_decide_eq_true_2; last done.
-        wp_op.
+      destruct (decide (n = 0%Z)); simplify_eq/=.
+      + wp_op.
         wp_if.
         done.
-      + rewrite bool_decide_eq_false_2; last done.
+      + rewrite bool_decide_eq_false_2; last congruence.
         wp_op.
         wp_if.
-        iInv (nroot .@ "ex3") as "I" "Hcl".
-        iDestruct "I" as (m) "[Hm Hl]".
+        iInv (nroot .@ "exercise3") as (m) ">[% Hl]".
         wp_store.
-        iMod ("Hcl" with "[Hl]") as "_".
-        { iNext. by iExists n; iFrame. }
-        iModIntro.
-        done.
-    - iIntros "!#" (w) "Hw".
+        iModIntro. iSplit.
+        * iExists n; auto with congruence.
+        * done.
+    - iIntros "!#" (? ->).
       wp_lam.
       wp_pures.
       iApply wp_assert.
+      (* Need because of atomic expression *)
       wp_bind (! _)%E.
-      iInv (nroot .@ "ex3") as "I" "Hcl".
-      iDestruct "I" as (m) "[#Hm Hl]".
+      iInv (nroot .@ "exercise3") as (m) ">[% Hl]".
       wp_load.
-      iMod ("Hcl" with "[Hl]") as "_".
-      { iNext. by iExists _; iFrame. }
-      iModIntro.
-      iDestruct "Hm" as %Hm.
+      iModIntro. iSplitL "Hl".
+      { iExists m; auto. }
       wp_op.
       rewrite bool_decide_eq_false_2; last done.
-      wp_op.
-      done.
+      by wp_op.
   Qed.
 
   Definition exercise4_prog : val :=
     λ: <>, let: "l" := ref #0 in λ: <>, "l" <- #true;; !"l".
 
-  Definition exercise4_ghost_auth `{!inG Σ (authUR (optionUR unitR))}
-             γ (o : option unit) := own γ (● o).
+  Section exercise4.
+    Context `{!inG Σ (authUR (optionUR unitR))}.
 
-  Definition exercise4_ghost_frag `{!inG Σ (authUR (optionUR unitR))}
-             γ (o : option unit) := own γ (◯ o).
+    Definition exercise4_auth (γ : gname) (b : bool) : iProp Σ :=
+      own γ (● (if b then Some () else None)).
 
-  Lemma exercise4_ghost_init `{!inG Σ (authUR (optionUR unitR))} :
-    (|==> ∃ γ, exercise4_ghost_auth γ None)%I.
-  Proof.
-    iApply own_alloc.
-    by apply auth_auth_valid.
-  Qed.
+    Definition exercise4_final (γ : gname) : iProp Σ :=
+      own γ (◯ (Some ())).
 
-  Lemma exercise4_ghost_update `{!inG Σ (authUR (optionUR unitR))} γ :
-    exercise4_ghost_auth γ None ==∗
-    exercise4_ghost_auth γ (Some ()) ∗ exercise4_ghost_frag γ (Some ()).
-  Proof.
-    iIntros "H".
-    iMod (own_update _ _ (● Some () ⋅ ◯ Some ()) with "H") as
-        "[$ $]"; last done.
-    apply auth_update_alloc.
-    by apply alloc_option_local_update.
-  Qed.
+    Lemma exercise4_ghost_init : (|==> ∃ γ, exercise4_auth γ false)%I.
+    Proof. iApply own_alloc. by apply auth_auth_valid. Qed.
 
-  Global Instance exercise4_ghost_frag_persistent
-         `{!inG Σ (authUR (optionUR unitR))} γ o :
-    Persistent (exercise4_ghost_frag γ o).
-  Proof. apply _. Qed.
+    Lemma exercise4_ghost_update γ b :
+      exercise4_auth γ b ==∗
+      exercise4_auth γ true ∗ exercise4_final γ.
+    Proof.
+      iIntros "H".
+      iMod (own_update _ _ (● Some () ⋅ ◯ Some ()) with "H") as "[$ $]"; last done.
+      apply auth_update_alloc. destruct b.
+      - by apply local_update_unital_discrete=> -[[]|].
+      - by apply alloc_option_local_update.
+    Qed.
 
-  Lemma exercise4_ghost_observe `{!inG Σ (authUR (optionUR unitR))} γ o :
-    exercise4_ghost_auth γ o ==∗
-    exercise4_ghost_auth γ o ∗ exercise4_ghost_frag γ o.
-  Proof.
-    iIntros "H".
-    iMod (own_update _ _ (● o ⋅ ◯ o) with "H") as "[$ $]"; last done.
-    apply auth_update_alloc.
-    apply local_update_unital_discrete.
-    intros ?. rewrite left_id. intros ? <-; split; first done.
-    by destruct o as [[]|].
-  Qed.
+    Global Instance exercise4_auth_timeless γ b : Timeless (exercise4_auth γ b).
+    Proof. apply _. Qed.
+    Global Instance exercise4_final_timeless γ : Timeless (exercise4_final γ).
+    Proof. apply _. Qed.
+    Global Instance exercise4_final_persistent γ : Persistent (exercise4_final γ).
+    Proof. apply _. Qed.
 
-  Lemma exercise4_ghost_agree `{!inG Σ (authUR (optionUR unitR))} γ o u :
-    exercise4_ghost_auth γ o -∗ exercise4_ghost_frag γ (Some u) -∗ ⌜o = Some u⌝.
-  Proof.
-    iIntros "H1 H2".
-    iDestruct (own_valid_2 with "H1 H2") as %[Hinc _]%auth_both_valid.
-    iPureIntro.
-    apply option_included in Hinc as [|(?&?&?&?&?)]; first done.
-    by destruct o as [[]|]; destruct u; simplify_eq.
-  Qed.
+    Lemma exercise4_ghost_agree γ b :
+      exercise4_auth γ b -∗ exercise4_final γ -∗ ⌜b = true⌝.
+    Proof.
+      iIntros "H1 H2".
+      iDestruct (own_valid_2 with "H1 H2") as %[Hinc _]%auth_both_valid.
+      apply option_included in Hinc as [|([]&[]&_&?&_)];
+        destruct b; naive_solver.
+    Qed.
 
-  Lemma exercise4 `{!inG Σ (authUR (optionUR unitR))} :
-    ∅ ⊨ exercise4_prog : sem_ty_unit → (sem_ty_unit → sem_ty_bool).
-  Proof.
-    iIntros (vs) "!# HΓ"; simpl.
-    iApply wp_value.
-    iIntros "!#" (v) "Hv".
-    wp_lam.
-    wp_alloc l as "Hl".
-    iMod exercise4_ghost_init as (γ) "Ho".
-    iMod (inv_alloc
-            (nroot .@ "ex4") _
-            (∃ o v, exercise4_ghost_auth γ o ∗ l ↦ v ∗
-                  ⌜match o with
-                  | None => v = #0
-                  | Some _ => v = #true
-                  end⌝
-         )%I with "[Hl Ho]") as "#Hinv".
-    { iNext. by iExists None, _; iFrame. }
-    wp_pures.
-    iIntros "!#" (w) "Hw".
-    wp_lam.
-    wp_bind (_ <- _)%E.
-    iInv (nroot .@ "ex4") as "I" "Hcl".
-    iDestruct "I" as (o x) "(Ho&Hl&Hx)".
-    wp_store.
-    destruct o.
-    - iMod (exercise4_ghost_observe with "Ho") as "[Ho #Hf]".
-      iMod ("Hcl" with "[Hl Ho]") as "_".
-      { iNext. by iExists _, _; iFrame. }
-      iModIntro.
+    Typeclasses Opaque exercise4_auth exercise4_final.
+
+    Lemma exercise4 :
+      ∅ ⊨ exercise4_prog : sem_ty_unit → (sem_ty_unit → sem_ty_bool).
+    Proof.
+      iIntros (vs) "!# HΓ"; simpl.
+      iApply wp_value.
+      iIntros "!#" (? ->).
+      wp_lam.
+      wp_alloc l as "Hl".
+      iMod exercise4_ghost_init as (γ) "Ho".
+      pose (I := (∃ b, exercise4_auth γ b ∗
+        l ↦ (if b then #true else #0))%I).
+      iMod (inv_alloc (nroot .@ "exercise4") _ I with "[Hl Ho]") as "#Hinv".
+      { iNext. iExists false. iFrame. }
       wp_pures.
-      iDestruct "Hx" as %->.
-      iInv (nroot .@ "ex4") as "I" "Hcl".
-      iDestruct "I" as (o x) "(Ho&Hl&Hx)".
-      wp_load.
-      iDestruct (exercise4_ghost_agree with "Ho Hf") as %->.
-      iDestruct "Hx" as %->.
-      iMod ("Hcl" with "[Hl Ho]") as "_".
-      { iNext. by iExists _, _; iFrame. }
-      iModIntro.
-      rewrite /sem_ty_car /=.
-      by iExists _.
-    - iMod (exercise4_ghost_update with "Ho") as "[Ho #Hf]".
-      iMod ("Hcl" with "[Hl Ho]") as "_".
-      { iNext. by iExists _, _; iFrame. }
-      iModIntro.
+      iIntros "!#" (? ->).
+      wp_lam.
+      (* Need because of atomic expression *)
+      wp_bind (_ <- _)%E.
+      iInv (nroot .@ "exercise4") as (o) ">[Ho Hl]".
+      wp_store.
+      iMod (exercise4_ghost_update with "Ho") as "[Ho Hf]".
+      iModIntro. iSplitL "Hl Ho".
+      { iNext. iExists true. iFrame. }
       wp_pures.
-      iDestruct "Hx" as %->.
-      iInv (nroot .@ "ex4") as "I" "Hcl".
-      iDestruct "I" as (o x) "(Ho&Hl&Hx)".
-      wp_load.
+      iInv (nroot .@ "exercise4") as (o') ">[Ho Hl]".
       iDestruct (exercise4_ghost_agree with "Ho Hf") as %->.
-      iDestruct "Hx" as %->.
-      iMod ("Hcl" with "[Hl Ho]") as "_".
-      { iNext. by iExists _, _; iFrame. }
-      iModIntro.
-      rewrite /sem_ty_car /=.
-      by iExists _.
-  Qed.
-
+      wp_load.
+      iModIntro. iSplitL "Hl Ho".
+      { iNext. iExists true. iFrame. }
+      rewrite /sem_ty_car /=. by iExists _.
+    Qed.
+  End exercise4.
 End exercises.
 
-Definition exercise5_prog (e : expr) (v : val) : expr := e ! v.
+(* REMOVE *) Definition exercise5_sem_ty Σ (v : val) : sem_ty Σ :=
+  SemTy (λ w, ⌜w = v⌝)%I.
 
-Definition exercise5_sem_ty Σ (v : val) : sem_ty Σ := SemTy (λ w, ⌜w = v⌝)%I.
-
-Lemma exercise5 `{!heapPreG Σ} e v σ w es σ' :
+Lemma exercise5 `{!heapPreG Σ} e (v : val) σ w es σ' :
   (∀ `{heapG Σ}, ∅ ⊨ e : ∀ A, A → A) →
-  rtc erased_step ([exercise5_prog e v : expr], σ) (of_val w :: es, σ') → w = v.
-Proof.
+  rtc erased_step ([e ! v]%E, σ) (of_val w :: es, σ') → w = v.
+(* REMOVE *) Proof.
   intros He.
-  apply sem_gen_type_safety with (φ := λ u, u = v).
-  intros ?.
-  exists (exercise5_sem_ty Σ v).
-  split.
-  - by iIntros (?) "?".
-  - iIntros (vs) "!# #Hvs".
-    iDestruct (env_sem_typed_empty with "Hvs") as %->.
-    iPoseProof (He with "Hvs") as "H"; simpl.
-    rewrite subst_map_empty.
-    wp_bind e.
-    iApply wp_wand_r; iSplitL; first eauto.
-    iIntros (u) "#Hu".
-    iSpecialize ("Hu" $! (exercise5_sem_ty Σ v)).
-    wp_bind (u #()).
-    iApply wp_wand_r; iSplitL; first eauto.
-    iIntros (u') "Hu'".
-    iApply "Hu'".
-    done.
+  apply sem_gen_type_safety with (φ := λ u, u = v)=> ?.
+  exists (exercise5_sem_ty Σ v). split.
+  { by iIntros (?) "?". }
+  iIntros (vs) "!# #Hvs".
+  iPoseProof (He with "Hvs") as "He /=".
+  wp_apply (wp_wand with "He").
+  iIntros (u) "#Hu".
+  iSpecialize ("Hu" $! (exercise5_sem_ty Σ v)).
+  wp_apply (wp_wand with "Hu"). iIntros (w') "Hw'". by iApply "Hw'".
 Qed.
